proof/invariant-abstract/ARM/ArchEmptyFail_AI.thy
@@ -119,6 +119,7 @@ context Arch begin global_naming ARM
 lemma preemption_point_empty_fail[wp, EmptyFail_AI_assms]:
   "empty_fail preemption_point"
   apply (wpsimp simp: mk_ef_def getActiveIRQ_def  preemption_point_def OR_choiceE_def andM_def
+                      commit_domain_time_def
                       ifM_def update_time_stamp_def getCurrentTime_def get_sc_active_def)
   done
 
