proof/invariant-abstract/BCorres_AI.thy
@@ -183,6 +183,7 @@ crunch_ignore (bcorres) (add: getActiveIRQ)
 lemma preemption_point_bcorres[wp]:
   "bcorres preemption_point preemption_point"
   unfolding preemption_point_def is_cur_domain_expired_def andM_def ifM_def get_sc_active_def
+            commit_domain_time_def
             update_time_stamp_def
   by wpsimp
 
