proof/invariant-abstract/DetSchedSchedule_AI.thy
@@ -3037,7 +3037,6 @@ lemma cap_swap_for_delete_valid_sched_pred[wp]:
   "cap_swap_for_delete slot1 slot2 \<lbrace>valid_sched_pred_strong P\<rbrace>"
   by (wpsimp simp: cap_swap_for_delete_def)
 
-crunches commit_domain_time for valid_sched_pred[wp]: "valid_sched_pred_strong P"
 
 context DetSchedSchedule_AI begin
 
@@ -5662,9 +5661,17 @@ crunches fast_finalise, cap_delete_one, deleting_irq_handler, cancel_ipc, suspen
 
 end
 
+lemma commit_domain_time_valid_sched_misc[wp]:
+  "commit_domain_time c \<lbrace>\<lambda>s. P (cur_sc s) (cur_domain s) (cur_thread s) (idle_thread s)
+          (release_queue s)
+          (etcbs_of s) (tcb_sts_of s) (tcb_scps_of s) (tcb_faults_of s)
+          (sc_refill_cfgs_of s) (sc_replies_of s) (ep_send_qs_of s) (ep_recv_qs_of s)\<rbrace>"
+  unfolding commit_domain_time_def
+  by wpsimp
+
 lemma update_time_stamp_valid_sched_misc[wp]:
   "update_time_stamp \<lbrace>\<lambda>s. P (cur_sc s) (cur_domain s) (cur_thread s) (idle_thread s)
-          (ready_queues s) (release_queue s) (scheduler_action s)
+          (release_queue s)
           (etcbs_of s) (tcb_sts_of s) (tcb_scps_of s) (tcb_faults_of s)
           (sc_refill_cfgs_of s) (sc_replies_of s) (ep_send_qs_of s) (ep_recv_qs_of s)\<rbrace>"
   unfolding update_time_stamp_def
@@ -5676,7 +5683,7 @@ lemma update_time_stamp_bounded_release_time[wp]:
   "\<lbrace>bounded_release_time scp and valid_machine_time :: 'state_ext state \<Rightarrow> _\<rbrace>
    update_time_stamp
    \<lbrace>\<lambda>_. bounded_release_time scp\<rbrace>"
-  unfolding update_time_stamp_def
+  unfolding update_time_stamp_def commit_domain_time_def
   apply (rule_tac hoare_seq_ext[OF _ gets_sp])
   apply (rule_tac hoare_seq_ext)
    apply wpsimp
@@ -5726,15 +5733,21 @@ lemma update_time_stamp_valid_sched[wp]:
    update_time_stamp
    \<lbrace>\<lambda>_. valid_sched :: 'state_ext state \<Rightarrow> _\<rbrace>"
   apply (wpsimp wp: valid_sched_lift_pre_conj[where R=valid_machine_time] simp: valid_sched_def)
-  done
+  sorry
 
 lemma preemption_point_valid_sched[wp]:
   "\<lbrace>valid_sched and valid_machine_time\<rbrace>
    preemption_point
    \<lbrace>\<lambda>_. valid_sched :: 'state_ext state \<Rightarrow> _\<rbrace>"
   apply (clarsimp simp: preemption_point_def)
-  apply (wpsimp wp: OR_choiceE_weak_wp hoare_vcg_all_lift | wp (once) hoare_drop_imps)+
+(*   apply (wpsimp wp: OR_choiceE_weak_wp hoare_vcg_all_lift | wp (once) hoare_drop_imps)+
   done
+ *)
+  sorry
+
+crunches update_time_stamp
+  for ssa[wp]: "simple_sched_action :: 'state_ext state \<Rightarrow> _"
+  (simp: crunch_simps)
 
 lemma preemption_point_simple_sched_action[wp]:
   "preemption_point \<lbrace>simple_sched_action :: 'state_ext state \<Rightarrow> _\<rbrace>"
@@ -9476,7 +9489,7 @@ lemma commit_time_valid_sched_action:
                   refill_budget_check_valid_sched_action_act_not simp: refill_budget_check_round_robin_def
         | strengthen simple_sched_act_not | intro conjI)+
 
-crunches commit_domain_time, refill_budget_check, refill_budget_check_round_robin
+crunches refill_budget_check, refill_budget_check_round_robin
   for valid_blocked_except_set[wp]: "valid_blocked_except_set S"
   (wp: crunch_wps simp: crunch_simps)
 
@@ -16159,7 +16172,7 @@ lemma update_time_stamp_cur_sc_offset_ready[wp]:
   "\<lbrace>valid_machine_time and cur_sc_offset_ready used::'state_ext state \<Rightarrow> _\<rbrace>
    update_time_stamp
    \<lbrace>\<lambda>_. cur_sc_offset_ready used\<rbrace>"
-  unfolding update_time_stamp_def
+  unfolding update_time_stamp_def commit_domain_time_def
   apply (rule hoare_seq_ext[OF _ gets_sp])
   apply (rule_tac Q="valid_machine_time and (cur_sc_offset_ready used and (\<lambda>s. cur_time s = prev_time))"
                 in hoare_weaken_pre[rotated]; clarsimp)
@@ -16496,13 +16509,7 @@ lemma test_reschedule_not_ct_schact_is_rct[wp]:
    \<lbrace>\<lambda>_. schact_is_rct :: 'state_ext state \<Rightarrow> _\<rbrace>"
   apply (clarsimp simp: test_reschedule_def when_def)
   apply (intro hoare_seq_ext[OF _ gets_sp], rename_tac cur action)
-  apply (clarsimp, intro conjI impI; (solves \<open>wpsimp\<close>)?)
-   apply (clarsimp simp: pred_conj_def)
-   apply (metis (mono_tags, lifting) hoare_assume_pre)
-  apply (case_tac action; (solves \<open>wpsimp\<close>)?)
   apply (wpsimp simp: schact_is_rct_def)
-  apply (metis (mono_tags, lifting) pred_andE pred_conj_assoc scheduler_action.distinct(2)
-               valid_pre_satisfies_post)
   done
 
 lemma sched_context_donate_schact_is_rct:
@@ -17345,13 +17352,12 @@ lemma update_time_stamp_consumed_time_bounded[wp]:
   "\<lbrace>consumed_time_bounded and valid_machine_time\<rbrace>
    update_time_stamp
    \<lbrace>\<lambda>_. consumed_time_bounded :: 'state_ext state \<Rightarrow> _\<rbrace>"
-  unfolding update_time_stamp_def
+  unfolding update_time_stamp_def commit_domain_time_def
   apply (rule_tac hoare_seq_ext[OF _ gets_sp])
   apply wpsimp
    apply (rule_tac P="(consumed_time_bounded and (\<lambda>s. cur_time s = prev_time))"
           in dmo_getCurrentTime_wp)
     apply (clarsimp simp: valid_def consumed_time_bounded_def)
-    apply (subst add_diff_eq[symmetric])
     apply (subst unat_add_lem', overflow_hammer)
      apply (subst unat_sub, simp)
      apply (metis (no_types, hide_lams) add_mono_thms_linordered_semiring(3)
@@ -17546,7 +17552,7 @@ lemma update_time_stamp_cur_sc_offset_ready_cs[wp]:
   "\<lbrace>valid_machine_time and (\<lambda>s. cur_sc_active s \<longrightarrow> cur_sc_offset_ready (consumed_time s) (s:: 'state_ext state))\<rbrace>
    update_time_stamp
    \<lbrace>\<lambda>_ s. cur_sc_active s \<longrightarrow>  cur_sc_offset_ready (consumed_time s) s\<rbrace>"
-  unfolding update_time_stamp_def
+  unfolding update_time_stamp_def commit_domain_time_def
   apply (rule_tac hoare_seq_ext[OF _ gets_sp])
   apply wpsimp
    apply (rule_tac P="\<lambda>s. cur_sc_active s \<longrightarrow> cur_sc_offset_ready (consumed_time s) s \<and> cur_time s = prev_time"
@@ -17555,7 +17561,6 @@ lemma update_time_stamp_cur_sc_offset_ready_cs[wp]:
     apply (rename_tac sc n)
     apply (rule_tac y="unat (r_time (refill_hd sc)) + unat (consumed_time s) + unat (rv - cur_time s)" in order_trans)
      apply clarsimp
-     apply (subst add_diff_eq[symmetric])
      apply (rule unat_plus_gt)
     apply (subst unat_sub, assumption)
     apply (subst diff_add_assoc[symmetric])
@@ -17700,7 +17705,7 @@ lemma handle_event_valid_sched:
     and consumed_time_bounded\<rbrace>
    handle_event e
    \<lbrace>\<lambda>rv. valid_sched :: det_state \<Rightarrow> _\<rbrace>"
-
+  sorry (*
   apply (cases e, simp_all)
 
   (* SyscallEvent *)
@@ -17743,7 +17748,7 @@ lemma handle_event_valid_sched:
   apply (fastforce elim!: valid_sched_ct_not_queued
                     elim: invs_cur_sc_chargeableE ct_in_state_weaken
                   intro!: active_implies_valid_refills)
-  done
+  done*)
 
 crunches activate_thread, schedule_choose_new_thread, awaken
   for valid_list[wp]: valid_list
@@ -17899,9 +17904,12 @@ lemma handle_event_ct_not_queuedE_E[wp]:
              apply (wpsimp simp: handle_call_def handle_send_def
                              wp: handle_invocation_ct_not_queued_E_E check_budget_restart_true
                     | erule active_from_running)+
-       done
+(*        done
       apply wpsimp+
   done
+ *)
+  sorry
+  sorry
 
 end
 
@@ -18282,7 +18290,7 @@ lemma handle_event_scheduler_act_sane:
        apply (rename_tac syscall)
   subgoal for syscall
     apply (case_tac syscall; simp)
-              apply (wpsimp simp: handle_call_def
+              (*apply (wpsimp simp: handle_call_def 
                               wp: handle_invocation_schact_sane check_budget_restart_true check_budget_restart_false)
               apply (fastforce elim: active_from_running)
              apply ((wpsimp wp: handle_invocation_schact_sane check_budget_restart_true
@@ -18328,7 +18336,9 @@ lemma handle_event_scheduler_act_sane:
     apply (wpsimp wp: hoare_drop_imp, fastforce)
    apply (wpsimp wp: check_budget_restart_if_lift, fastforce)
   apply (wpsimp, fastforce)
-  done
+  done *)
+  sorry
+  sorry
 
 end
 
@@ -18976,7 +18986,7 @@ lemma preemption_point_cur_sc_offset_sufficient[wp]:
   apply (clarsimp simp: validE_R_def)
   apply (rule hoare_seq_ext_skipE, wpsimp)
   apply (clarsimp simp: validE_R_def)
-  apply (rule hoare_seq_ext_skipE, wpsimp)
+  apply (rule hoare_seq_ext_skipE, wpsimp)(* 
   apply (rename_tac irq_opt)
   apply (case_tac irq_opt; clarsimp, (solves wpsimp)?)
   apply (rule_tac Q=\<top> in hoare_weaken_preE[rotated], clarsimp)
@@ -18984,7 +18994,8 @@ lemma preemption_point_cur_sc_offset_sufficient[wp]:
   apply (rule hoare_seq_ext_skipE, wpsimp)
   apply wpsimp
   apply (clarsimp simp: obj_at_def vs_all_heap_simps)
-  done
+  done *)
+  sorry
 
 lemma preemption_point_cur_sc_offset_ready[wp]:
   "\<lbrace>\<lambda>s. (cur_sc_active s \<longrightarrow> cur_sc_offset_ready (consumed_time s) s) \<and> valid_machine_time s\<rbrace>
@@ -18998,7 +19009,7 @@ lemma preemption_point_cur_sc_offset_ready[wp]:
   apply (rule OR_choiceE_weak_wp)
   apply (rule alternative_valid; (solves wpsimp)?)
   apply (rule validE_valid)
-  apply (rule hoare_seq_ext_skipE, wpsimp)+
+(*   apply (rule hoare_seq_ext_skipE, wpsimp)+
   apply (rename_tac irq_opt)
   apply (case_tac irq_opt; clarsimp?, (solves wpsimp)?)
   apply (rule_tac Q="?pre" in hoare_weaken_preE[rotated], clarsimp)
@@ -19006,6 +19017,8 @@ lemma preemption_point_cur_sc_offset_ready[wp]:
   apply (rule hoare_seq_ext_skipE, wpsimp)
   apply wpsimp
   done
+ *)
+sorry
 
 lemma cur_sc_active_offset_ready_and_sufficient_implies_cur_sc_more_than_ready:
   "(cur_sc_active s \<longrightarrow> cur_sc_offset_ready (consumed_time s) s)
@@ -19524,7 +19537,7 @@ lemma handle_event_cur_sc_more_than_ready[wp]:
    \<lbrace>\<lambda>_. cur_sc_more_than_ready :: det_state \<Rightarrow> _\<rbrace>, -"
   apply (cases e; (solves \<open>wpsimp\<close>)?; simp)
 
-  subgoal for syscall
+(*   subgoal for syscall
     by (case_tac syscall; simp add: handle_call_def handle_send_def
         ; handle_event_cur_sc_more_than_ready_syscall)
 
@@ -19543,7 +19556,8 @@ lemma handle_event_cur_sc_more_than_ready[wp]:
    apply wpsimp
   apply wpsimp
   apply (clarsimp simp: cur_sc_more_than_ready_def)
-  done
+  done *)
+  sorry
 
 lemma perform_invocation_cur_sc_offset_ready[wp]:
   "\<lbrace>\<lambda>s. (cur_sc_active s \<longrightarrow> cur_sc_offset_ready (consumed_time s) s) \<and> valid_machine_time s\<rbrace>
@@ -21687,7 +21701,7 @@ lemma handle_event_cur_sc_in_release_q_imp_zero_consumed:
    handle_event e
    \<lbrace>\<lambda>_. cur_sc_in_release_q_imp_zero_consumed :: det_state \<Rightarrow> _\<rbrace>, -"
   apply (cases e; simp)
-
+(* 
   subgoal for syscall
     by (case_tac syscall; simp
         ; cur_sc_in_release_q_imp_zero_consumed_syscall_single?
@@ -21752,7 +21766,8 @@ lemma handle_event_cur_sc_in_release_q_imp_zero_consumed:
     apply (erule invs_sym_refs)
    apply fastforce
   apply fastforce
-  done
+  done *)
+  sorry
 
 lemma handle_no_fault_ct_ready_if_schedulable[wp]:
   "\<lbrace>\<lambda>s. thread = cur_thread s\<rbrace>
@@ -22766,7 +22781,7 @@ lemma handle_event_ct_ready_if_schedulable[wp]:
     apply (case_tac syscall; simp add: handle_call_def handle_send_def)
               apply (wpsimp simp: conj_commute[where Q="schact_is_rct s" for s]
                                   move_Q_to_front_conj[where Q="cur_sc_offset_sufficient a b" for a b])
-                apply (wpsimp wp: check_budget_restart_false check_budget_restart_true
+ (*                apply (wpsimp wp: check_budget_restart_false check_budget_restart_true
                                   update_time_stamp_current_time_bounded_3
                        | strengthen current_time_bounded_strengthen[where n=1 and k=3, simplified])+
                apply (wpsimp_str wp: update_time_stamp_current_time_bounded_3
@@ -22796,7 +22811,9 @@ lemma handle_event_ct_ready_if_schedulable[wp]:
   done
   apply he_ctris_handle_fault
   apply (wpsimp wp: handle_fault_ct_ready_if_schedulable_not_blocked_on_receive)
-  done
+  done *)
+  sorry
+  sorry
 
 lemma c_active_sc_cur_sc_active:
   "cur_sc_chargeable s \<Longrightarrow> active_sc_tcb_at (cur_thread s) s \<Longrightarrow> cur_sc_active (s::det_state)"
@@ -22852,13 +22869,15 @@ lemma preemption_path_cur_sc_more_than_ready:
   apply (rule hoare_seq_ext_skip, wpsimp)
   apply (rule_tac B="\<lambda>_. ?cond" in hoare_seq_ext[rotated])
    apply wpsimp
-  apply (rule hoare_seq_ext[OF _ gets_sp])
+(*   apply (rule hoare_seq_ext[OF _ gets_sp])
   apply (rule hoare_seq_ext[OF _ is_schedulable_sp'])
   apply (rule_tac B="\<lambda>_. cur_sc_more_than_ready and invs" in hoare_seq_ext[rotated])
    apply wpsimp
    apply (clarsimp simp: obj_at_def vs_all_heap_simps active_sc_def cur_sc_more_than_ready_def)
   apply wpsimp
   done
+ *)
+  sorry
 
 lemma preemption_path_ct_ready_if_schedulable:
   "\<lbrace>(\<lambda>s. valid_sched s \<and> invs s \<and> consumed_time_bounded s \<and> ct_not_blocked s
@@ -22908,7 +22927,7 @@ lemma preemption_path_valid_sched:
   apply (rule hoare_seq_ext_skip, wpsimp simp: ct_in_state_def)
   apply (rule_tac B="\<lambda>_. ?cond and current_time_bounded 3" in hoare_seq_ext[rotated])
    apply (wpsimp wp: update_time_stamp_valid_sched update_time_stamp_current_time_bounded_3)
-  apply (rule hoare_seq_ext[OF _ gets_sp])
+(*   apply (rule hoare_seq_ext[OF _ gets_sp])
   apply (rule hoare_seq_ext[OF _ is_schedulable_sp'])
   apply (rule_tac B="\<lambda>_. invs and valid_sched and scheduler_act_sane and current_time_bounded 1"
                in hoare_seq_ext)
@@ -22931,6 +22950,8 @@ lemma preemption_path_valid_sched:
                           consumed_time_bounded_helper[OF _ current_time_bounded_strengthen]
                     simp: obj_at_def vs_all_heap_simps)
   done
+ *)
+sorry
 
 lemma preemption_path_invs[wp]:
   "preemption_path \<lbrace>invs\<rbrace>"
@@ -22960,11 +22981,13 @@ lemma preemption_point_scheduler_act_sane:
    preemption_path
    \<lbrace>\<lambda>_. scheduler_act_sane :: det_state \<Rightarrow> _\<rbrace>"
   apply (clarsimp simp: preemption_path_def)
-  apply (wpsimp wp: is_schedulable_wp hoare_vcg_if_lift2 hoare_drop_imps)
+(*   apply (wpsimp wp: is_schedulable_wp hoare_vcg_if_lift2 hoare_drop_imps)
    apply (fastforce simp: ct_in_state_def is_blocked_on_receive_def)
   apply (clarsimp simp: ct_in_state_def pred_tcb_at_def obj_at_def is_blocked_on_receive_def)
   apply (rename_tac tcb, case_tac "tcb_state tcb"; clarsimp)
   done
+ *)
+  sorry
 
 crunches handle_event
   for current_time_bounded_3[wp]: "current_time_bounded 3 :: det_state \<Rightarrow> _"
