proof/invariant-abstract/Untyped_AI.thy
@@ -2778,8 +2778,8 @@ lemma reset_untyped_cap_invs_etc:
       in mapME_x_validE_nth)
      apply (rule hoare_pre)
       apply (wp set_untyped_cap_invs_simple
-                set_cap_no_overlap set_cap_cte_wp_at
-                preemption_point_inv
+                set_cap_no_overlap set_cap_cte_wp_at preemption_point_invE_E
+                preemption_point_invE_R
                 hoare_vcg_ex_lift hoare_vcg_const_imp_lift
                 hoare_vcg_const_Ball_lift set_cap_cte_cap_wp_to
                 | strengthen empty_descendants_range_in
@@ -2787,14 +2787,8 @@ lemma reset_untyped_cap_invs_etc:
                 | rule irq_state_independent_A_conjI
                 | simp add: cte_wp_at_caps_of_state
                 | wp (once) ct_in_state_thread_state_lift
-                | (rule irq_state_independent_A_def[THEN meta_eq_to_obj_eq, THEN iffD2]
-                        getCurrentTime_independent_A_def[THEN meta_eq_to_obj_eq, THEN iffD2]
-                        time_state_independent_A_def[THEN meta_eq_to_obj_eq, THEN iffD2]
-                        cur_time_independent_A_def[THEN meta_eq_to_obj_eq, THEN iffD2]
-                        update_time_stamp_independent_A_def[THEN meta_eq_to_obj_eq, THEN iffD2],
-                  simp add: ex_cte_cap_wp_to_def ct_in_state_def))+
-     apply (simp add: ct_in_state_def ex_cte_cap_wp_to_def cte_wp_at_caps_of_state)
-     apply clarsimp
+                | (clarsimp simp: ct_in_state_def ex_cte_cap_wp_to_def)
+                | rule conj_cong)+
        apply (clarsimp simp: is_aligned_neg_mask_eq bits_of_def field_simps
                            cte_wp_at_caps_of_state nth_rev)
      apply (strengthen order_trans[where z="2 ^ sz", rotated, mk_strg I E])
@@ -2818,7 +2812,7 @@ lemma reset_untyped_cap_obj_at:
          reset_untyped_cap slot
          \<lbrace>\<lambda>_ s. P (obj_at P' p s)\<rbrace>"
   apply (wpsimp wp: set_cap.cspace_agnostic_obj_at[OF assms] mapME_x_inv_wp
-                    preemption_point_inv get_cap_wp
+                    preemption_point_inv get_cap_wp update_time_stamp_inv
               simp: reset_untyped_cap_def delete_objects_def)
   by (case_tac cap; fastforce simp: cte_wp_at_caps_of_state bits_of_def)
 
